theories/program_logic/weakestpre.v
@@ -405,22 +405,22 @@ Section proofmode_classes.
     AddModal (|={E}=> P) P (WP e @ s; E {{ Φ }}).
   Proof. by rewrite /AddModal fupd_frame_r wand_elim_r fupd_wp. Qed.
 
-  Global Instance acc_elim_wp {X} E1 E2 α β γ e s Φ :
+  Global Instance elim_acc_wp {X} E1 E2 α β γ e s Φ :
     Atomic (stuckness_to_atomicity s) e →
-    AccElim (X:=X) E1 E2 α β γ (WP e @ s; E1 {{ Φ }})
+    ElimAcc (X:=X) E1 E2 α β γ (WP e @ s; E1 {{ Φ }})
             (λ x, WP e @ s; E2 {{ v, |={E2}=> β x ∗ coq_tactics.maybe_wand (γ x) (Φ v) }})%I.
   Proof.
-    intros ?. rewrite /AccElim. setoid_rewrite coq_tactics.maybe_wand_sound.
+    intros ?. rewrite /ElimAcc. setoid_rewrite coq_tactics.maybe_wand_sound.
     iIntros "Hinner >Hacc". iDestruct "Hacc" as (x) "[Hα Hclose]".
     iApply (wp_wand with "[Hinner Hα]"); first by iApply "Hinner".
     iIntros (v) ">[Hβ HΦ]". iApply "HΦ". by iApply "Hclose".
   Qed.
 
-  Global Instance acc_elim_wp_nonatomic {X} E α β γ e s Φ :
-    AccElim (X:=X) E E α β γ (WP e @ s; E {{ Φ }})
+  Global Instance elim_acc_wp_nonatomic {X} E α β γ e s Φ :
+    ElimAcc (X:=X) E E α β γ (WP e @ s; E {{ Φ }})
             (λ x, WP e @ s; E {{ v, |={E}=> β x ∗ coq_tactics.maybe_wand (γ x) (Φ v) }})%I.
   Proof.
-    rewrite /AccElim. setoid_rewrite coq_tactics.maybe_wand_sound.
+    rewrite /ElimAcc. setoid_rewrite coq_tactics.maybe_wand_sound.
     iIntros "Hinner >Hacc". iDestruct "Hacc" as (x) "[Hα Hclose]".
     iApply wp_fupd.
     iApply (wp_wand with "[Hinner Hα]"); first by iApply "Hinner".
